tests/overloading/strict/StrictBool.fst
@@ -1,2 +1,5 @@
 module StrictBool
 let f (x:bool) : bool = x
+
+(* See StrictInt.same. *)
+let same : int = 1
